ReTierStaticSemantics.v
@@ -1,9 +1,6 @@
 Require Import ReTierSyntax.
 Require Import Maps.
 
-(*
-Definition idMap := 
-*)
 
 (** Typing environment for reactives, named Psi in informal specification. **)
 Definition reactEnv := partial_map r T.
@@ -30,19 +27,19 @@ Definition emptyVarEnv: varEnv := idEmpty.
  ----------------------------------------------------------------------------
 **)
 
-Reserved Notation "peerTyping ; Ties ; Psi ; Delta ; Gamma ; P |- t : T"
+Reserved Notation "program :: Psi ; Delta ; Gamma ; P |- t : T"
   (at level 40,
-   Ties at next level, Psi at next level, Delta at next level,
-   Gamma at next level, P at next level, t at next level).
+   Psi at next level, Delta at next level, Gamma at next level,
+   P at next level, t at next level).
 
-Reserved Notation "peerTyping ; Ties ; Psi ; Delta |- s"
-  (at level 40, Ties at next level, Psi at next level, Delta at next level).
+Reserved Notation "program :: Psi ; Delta |- s"
+  (at level 40, Psi at next level, Delta at next level).
 
 
 
 (** auxiliary functions for aggegation **)
 
-  Definition phi (ties: Ties) (p0 p1: P) (type: T) :=
+  Definition phi (ties: ties) (p0 p1: P) (type: T) :=
     match ties (p0, p1) with
     | Some multiple => Some (List type)
     | Some optional => Some (Option type)
@@ -55,127 +52,120 @@ Reserved Notation "peerTyping ; Ties ; Psi ; Delta |- s"
 
 (* --------------------------------------------------------------------- *)
 
-Definition areTied (ties: Ties) (p1 p2: P): bool :=
-  match ties (p1, p2) with
-  | None        => false
-  | Some mNone  => false
-  | Some _      => true
-  end.
 
 
-
-Inductive typing_t : peerTyping -> Ties -> reactEnv -> placeEnv -> varEnv -> P -> t -> T -> Prop :=
+Inductive typing_t : program -> reactEnv -> placeEnv -> varEnv -> P -> t -> T -> Prop :=
 
   (* rules for local evaluation *)
 
-  | T_Var: forall peerTyping ties Psi Delta Gamma P x T,
+  | T_Var: forall program Psi Delta Gamma P x T,
       Gamma x = Some T \/ Gamma x = None /\ Delta x = Some (T on P) ->
-      peerTyping; ties; Psi; Delta; Gamma; P |- (idApp x) : T
+      program :: Psi; Delta; Gamma; P |- (idApp x) : T
 
-  | T_App: forall peerTyping ties Psi Delta Gamma P t1 t2 T1 T2,
-      peerTyping; ties; Psi; Delta; Gamma; P |- t1 : T2 ~> T1 ->
-      peerTyping; ties; Psi; Delta; Gamma; P |- t2 : T2 ->
-      peerTyping; ties; Psi; Delta; Gamma; P |- app t1 t2 : T1
+  | T_App: forall program Psi Delta Gamma P t1 t2 T1 T2,
+      program :: Psi; Delta; Gamma; P |- t1 : T2 ~> T1 ->
+      program :: Psi; Delta; Gamma; P |- t2 : T2 ->
+      program :: Psi; Delta; Gamma; P |- app t1 t2 : T1
 
-  | T_Abs: forall peerTyping ties Psi Delta Gamma P x t T1 T2,
-      peerTyping; ties; Psi; Delta; idUpdate x T1 Gamma; P |- t : T2 ->
-      peerTyping; ties; Psi; Delta; Gamma; P |- lambda x T1 t : T1 ~> T2
+  | T_Abs: forall program Psi Delta Gamma P x t T1 T2,
+      program :: Psi; Delta; idUpdate x T1 Gamma; P |- t : T2 ->
+      program :: Psi; Delta; Gamma; P |- lambda x T1 t : T1 ~> T2
 
-  | T_Cons: forall peerTyping ties Psi Delta Gamma P t0 t1 T,
-      peerTyping; ties; Psi; Delta; Gamma; P |- t0 : T ->
-      peerTyping; ties; Psi; Delta; Gamma; P |- t1 : List T ->
-      peerTyping; ties; Psi; Delta; Gamma; P |- cons t0 t1 : List T
+  | T_Cons: forall program Psi Delta Gamma P t0 t1 T,
+      program :: Psi; Delta; Gamma; P |- t0 : T ->
+      program :: Psi; Delta; Gamma; P |- t1 : List T ->
+      program :: Psi; Delta; Gamma; P |- cons t0 t1 : List T
 
-  | T_Nil: forall peerTyping ties Psi Delta Gamma P T,
-      peerTyping; ties; Psi; Delta; Gamma; P |- nil T : List T
+  | T_Nil: forall program Psi Delta Gamma P T,
+      program :: Psi; Delta; Gamma; P |- nil T : List T
 
-  | T_Some: forall peerTyping ties Psi Delta Gamma P t T,
-      peerTyping; ties; Psi; Delta; Gamma; P |- t : T ->
-      peerTyping; ties; Psi; Delta; Gamma; P |- some t : Option T
+  | T_Some: forall program Psi Delta Gamma P t T,
+      program :: Psi; Delta; Gamma; P |- t : T ->
+      program :: Psi; Delta; Gamma; P |- some t : Option T
 
-  | T_None: forall peerTyping ties Psi Delta Gamma P T,
-      peerTyping; ties; Psi; Delta; Gamma; P |- none T : Option T
+  | T_None: forall program Psi Delta Gamma P T,
+      program :: Psi; Delta; Gamma; P |- none T : Option T
 
-  | T_Unit: forall peerTyping ties Psi Delta Gamma P,
-      peerTyping; ties; Psi; Delta; Gamma; P |- unit : Unit
+  | T_Unit: forall program Psi Delta Gamma P,
+      program :: Psi; Delta; Gamma; P |- unit : Unit
 
   (* rules for remote access *)
 
-  | T_Peer: forall peerTyping ties Psi Delta Gamma P0 P1 p,
-      peerTyping p = Some P1 ->
-      peerTyping; ties; Psi; Delta; Gamma; P0 |- peerApp p : Remote P1
+  | T_Peer: forall program Psi Delta Gamma P0 P1 p,
+      peer_instance_type program p = Some P1 ->
+      program :: Psi; Delta; Gamma; P0 |- peerApp p : Remote P1
 
-  | T_AsLocal: forall peerTyping ties Psi Delta Gamma P0 P1 t T0 T1,
+  | T_AsLocal: forall program Psi Delta Gamma P0 P1 t T0 T1,
       transmittable_type T1 ->
-      peerTyping; ties; Psi; Delta; emptyVarEnv; P1 |- t : T1 ->
-      areTied ties P0 P1 = true ->
-      phi ties P0 P1 T1 = Some T0 ->
-      peerTyping; ties; Psi; Delta; Gamma; P0 |- asLocal t (T1 on P1) : T0
+      program :: Psi; Delta; emptyVarEnv; P1 |- t : T1 ->
+      are_peers_tied program P0 P1 ->
+      phi (peer_ties program) P0 P1 T1 = Some T0 ->
+      program :: Psi; Delta; Gamma; P0 |- asLocal t (T1 on P1) : T0
 
-  | T_AsLocalFrom: forall peerTyping ties Psi Delta Gamma P0 P1 t0 t1 T,
+  | T_AsLocalFrom: forall program Psi Delta Gamma P0 P1 t0 t1 T,
       transmittable_type T ->
-      peerTyping; ties; Psi; Delta; emptyVarEnv; P1 |- t0 : T ->
-      areTied ties P0 P1 = true ->
-      peerTyping; ties; Psi; Delta; Gamma; P0 |- t1 : Remote P1 ->
-      peerTyping; ties; Psi; Delta; Gamma; P0 |- asLocalFrom t0 (T on P1) t1 : T
+      program :: Psi; Delta; emptyVarEnv; P1 |- t0 : T ->
+      are_peers_tied program P0 P1 ->
+      program :: Psi; Delta; Gamma; P0 |- t1 : Remote P1 ->
+      program :: Psi; Delta; Gamma; P0 |- asLocalFrom t0 (T on P1) t1 : T
 
-  | T_Comp: forall peerTyping ties Psi Delta Gamma P0 P1 x t0 t1 T0 T1 T2,
+  | T_Comp: forall program Psi Delta Gamma P0 P1 x t0 t1 T0 T1 T2,
       transmittable_type T1 ->
       transmittable_type T0 ->
-      peerTyping; ties; Psi; Delta; Gamma; P0 |- t0 : T0 ->
-      peerTyping; ties; Psi; Delta; idUpdate x T0 emptyVarEnv; P1 |- t1 : T1 ->
-      areTied ties P0 P1 = true ->
-      phi ties P0 P1 T1 = Some T2 ->
-      peerTyping; ties; Psi; Delta; Gamma; P0 |- asLocalIn x t0 t1 (T1 on P1) : T2
+      program :: Psi; Delta; Gamma; P0 |- t0 : T0 ->
+      program :: Psi; Delta; idUpdate x T0 emptyVarEnv; P1 |- t1 : T1 ->
+      are_peers_tied program P0 P1 ->
+      phi (peer_ties program) P0 P1 T1 = Some T2 ->
+      program :: Psi; Delta; Gamma; P0 |- asLocalIn x t0 t1 (T1 on P1) : T2
 
-  | T_ComFrom: forall peerTyping ties Psi Delta Gamma P0 P1 x t0 t1 t2 T0 T1,
+  | T_ComFrom: forall program Psi Delta Gamma P0 P1 x t0 t1 t2 T0 T1,
       transmittable_type T1 ->
       transmittable_type T0 ->
-      peerTyping; ties; Psi; Delta; Gamma; P0 |- t0 : T0 ->
-      peerTyping; ties; Psi; Delta; idUpdate x T0 emptyVarEnv; P1 |- t1 : T1 ->
-      areTied ties P0 P1 = true ->
-      peerTyping; ties; Psi; Delta; Gamma; P0 |- t2 : Remote P1 ->
-      peerTyping; ties; Psi; Delta; Gamma; P0 |- asLocalInFrom x t0 t1 (T1 on P1) t2 : T1
+      program :: Psi; Delta; Gamma; P0 |- t0 : T0 ->
+      program :: Psi; Delta; idUpdate x T0 emptyVarEnv; P1 |- t1 : T1 ->
+      are_peers_tied program P0 P1 ->
+      program :: Psi; Delta; Gamma; P0 |- t2 : Remote P1 ->
+      program :: Psi; Delta; Gamma; P0 |- asLocalInFrom x t0 t1 (T1 on P1) t2 : T1
 
   (* rules for reactives *)
 
-  | T_Reactive: forall peerTyping ties Psi Delta Gamma P r T,
+  | T_Reactive: forall program Psi Delta Gamma P r T,
       Psi r = Some T -> 
-      peerTyping; ties; Psi; Delta; Gamma; P |- reactApp r : T
+      program :: Psi; Delta; Gamma; P |- reactApp r : T
 
-  | T_Signal: forall peerTyping ties Psi Delta Gamma P t T,
-      peerTyping; ties; Psi; Delta; Gamma; P |- t : T ->
-      peerTyping; ties; Psi; Delta; Gamma; P |- signal t : Signal T
+  | T_Signal: forall program Psi Delta Gamma P t T,
+      program :: Psi; Delta; Gamma; P |- t : T ->
+      program :: Psi; Delta; Gamma; P |- signal t : Signal T
 
-  | T_ReactiveVar: forall peerTyping ties Psi Delta Gamma P t T,
-      peerTyping; ties; Psi; Delta; Gamma; P |- t : T ->
-      peerTyping; ties; Psi; Delta; Gamma; P |- var t : Var T
+  | T_ReactiveVar: forall program Psi Delta Gamma P t T,
+      program :: Psi; Delta; Gamma; P |- t : T ->
+      program :: Psi; Delta; Gamma; P |- var t : Var T
 
-  | T_Now: forall peerTyping ties Psi Delta Gamma P t T1 T0,
-      peerTyping; ties; Psi; Delta; Gamma; P |- t : T0 ->
+  | T_Now: forall program Psi Delta Gamma P t T1 T0,
+      program :: Psi; Delta; Gamma; P |- t : T0 ->
       T0 = Signal T1 \/ T0 = Var T1 ->
-      peerTyping; ties; Psi; Delta; Gamma; P |- now t : T1
+      program :: Psi; Delta; Gamma; P |- now t : T1
 
-  | T_Set: forall peerTyping ties Psi Delta Gamma P t1 t2 T,
-      peerTyping; ties; Psi; Delta; Gamma; P |- t1 : Var T ->
-      peerTyping; ties; Psi; Delta; Gamma; P |- t2 : T ->
-      peerTyping; ties; Psi; Delta; Gamma; P |- set t1 t2 : Unit
+  | T_Set: forall program Psi Delta Gamma P t1 t2 T,
+      program :: Psi; Delta; Gamma; P |- t1 : Var T ->
+      program :: Psi; Delta; Gamma; P |- t2 : T ->
+      program :: Psi; Delta; Gamma; P |- set t1 t2 : Unit
 
-  | T_Nat: forall peerTyping ties Psi Delta Gamma P n,
-      peerTyping; ties; Psi; Delta; Gamma; P |- tnat n : Tnat
+  | T_Nat: forall program Psi Delta Gamma P n,
+      program :: Psi; Delta; Gamma; P |- tnat n : Tnat
 
-where "peerTyping ; Ties ; Psi ; Delta ; Gamma ; P |- t : T" := (typing_t peerTyping Ties Psi Delta Gamma P t T).
+where "program :: Psi ; Delta ; Gamma ; P |- t : T" := (typing_t program Psi Delta Gamma P t T).
 
 
-Inductive typing_s : peerTyping -> Ties -> reactEnv -> placeEnv -> s -> Prop :=
-  | T_End: forall peerTyping ties Psi Delta,
-      peerTyping; ties; Psi; Delta |- pUnit
+Inductive typing_s : program -> reactEnv -> placeEnv -> s -> Prop :=
+  | T_End: forall program Psi Delta,
+      program :: Psi; Delta |- pUnit
 
-  | T_Place: forall peerTyping ties Psi Delta x t s T P,
-      peerTyping; ties; Psi; idUpdate x (T on P) Delta |- s ->
-      peerTyping; ties; Psi; Delta; emptyVarEnv; P |- t : T ->
-      peerTyping; ties; Psi; Delta |- placed x (T on P) t s
+  | T_Place: forall program Psi Delta x t s T P,
+      program :: Psi; idUpdate x (T on P) Delta |- s ->
+      program :: Psi; Delta; emptyVarEnv; P |- t : T ->
+      program :: Psi; Delta |- placed x (T on P) t s
 
-where "peerTyping ; Ties ; Psi ; Delta |- s" := (typing_s peerTyping Ties Psi Delta s).
+where "program :: Psi ; Delta |- s" := (typing_s program Psi Delta s).
 
 
