Test_ReTierStaticSemantics.v
@@ -19,36 +19,26 @@ Require Import ReTierSyntax.
 Definition testPsi1: reactEnv   := reactUpdate (Reactive 0) Unit reactEmpty.
 Definition testGamma1: varEnv   := idUpdate (Id "x") Tnat (idUpdate (Id "y") Unit idEmpty).
 Definition testDelta1: placeEnv := idUpdate (Id "x") (Unit on (Peer "px")) idEmpty.
-Definition testTies1  :=  (tie_update (Peer "p0" *-> Peer "pm")
-                            (tie_update (Peer "p0" ?-> Peer "po")
-                              (tie_update (Peer "p0" S-> Peer "ps")
-                                (tie_update ((Peer "p0") N-> (Peer "pn"))
-                                  noTies)))).
-Definition testPeerTyping1 := (pT_update (PeerInst 4) (Peer "pm")
-                                (pT_update (PeerInst 3) (Peer "po")
-                                  (pT_update (PeerInst 2) (Peer "ps")
-                                    (pT_update (PeerInst 1) (Peer "pn")
-                                      (pT_update (PeerInst 0) (Peer "p0")
-                                      noPeers))))).
-
+Definition testTies1  := Ties ["p0" *-> "pm", "p0" ?-> "po", "p0" S-> "ps", "p0" N-> "pn"].
+Definition testPeerTyping1 := TypedInstances [4 : "pm", 3 : "po", 2 : "ps", 1 : "pn", 0 : "p0"].
 
 Example test_pltIsWellTyped_TEnd_1:
-  noPeers; noTies; emptyReactEnv; emptyPlaceEnv |- pUnit.
+  (Program NoTies NoTypedInstances) :: emptyReactEnv; emptyPlaceEnv |- pUnit.
 Proof. apply T_End. Qed.
 
 
 Example test_pltIsWellTyped_TEnd_2:
-  noPeers; noTies; testPsi1; testDelta1 |- pUnit.
+  (Program NoTies NoTypedInstances) :: testPsi1; testDelta1 |- pUnit.
 Proof. apply T_End. Qed.
 
 
 Example test_hasType_TUnit_1:
-  noPeers; noTies; emptyReactEnv; emptyPlaceEnv; emptyVarEnv; Peer "dummy" |- unit : Unit.
+  (Program NoTies NoTypedInstances) :: emptyReactEnv; emptyPlaceEnv; emptyVarEnv; Peer "dummy" |- unit : Unit.
 Proof. apply T_Unit. Qed.
 
 
 Example test_pltIsWellTyped_TPlace_1:
-  noPeers; noTies; testPsi1; testDelta1 |- placed (Id "x") (Unit on (Peer "px")) unit pUnit.
+  (Program NoTies NoTypedInstances) :: testPsi1; testDelta1 |- placed (Id "x") (Unit on (Peer "px")) unit pUnit.
 Proof.
   apply T_Place.
   - apply T_End.
@@ -57,33 +47,33 @@ Qed.
 
 
 Example test_hasType_TVar_normalVar_1:
-  noPeers; noTies; emptyReactEnv; emptyPlaceEnv; testGamma1; Peer "p1" |- idApp (Id "x") : Tnat.
+  (Program NoTies NoTypedInstances) :: emptyReactEnv; emptyPlaceEnv; testGamma1; Peer "p1" |- idApp (Id "x") : Tnat.
 Proof. apply T_Var. left. reflexivity. Qed.
 
 
 Example test_hasType_TVar_placedVar_2:
-  noPeers; noTies; emptyReactEnv; testDelta1; emptyVarEnv; Peer "px" |- idApp (Id "x") : Unit.
+  (Program NoTies NoTypedInstances) :: emptyReactEnv; testDelta1; emptyVarEnv; Peer "px" |- idApp (Id "x") : Unit.
 Proof. apply T_Var. right. split. - reflexivity. - reflexivity. Qed.
 
 
 Example test_hasType_TAbs_1: 
-    noPeers; noTies; emptyReactEnv; emptyPlaceEnv; emptyVarEnv; Peer "dummy" |- lambda (Id "x") Tnat unit : Tnat ~> Unit.
+    (Program NoTies NoTypedInstances) :: emptyReactEnv; emptyPlaceEnv; emptyVarEnv; Peer "dummy" |- lambda (Id "x") Tnat unit : Tnat ~> Unit.
 Proof. apply T_Abs. apply T_Unit. Qed.
 
 
 Example test_hasType_TAbs_2: 
-    noPeers; noTies; emptyReactEnv; emptyPlaceEnv; emptyVarEnv; Peer "dummy" |- lambda (Id "x") Tnat (idApp (Id "x")) : Tnat ~> Tnat.
+    (Program NoTies NoTypedInstances) :: emptyReactEnv; emptyPlaceEnv; emptyVarEnv; Peer "dummy" |- lambda (Id "x") Tnat (idApp (Id "x")) : Tnat ~> Tnat.
 Proof. apply T_Abs. apply T_Var. left. reflexivity. Qed.
 
 
 (** Tests variable shadowing **)
 Example test_hasType_TAbs_3:
-  noPeers; noTies; emptyReactEnv; emptyPlaceEnv; testGamma1; Peer "_" |- lambda (Id "x") Unit (idApp (Id "x")) : Unit ~> Unit.
+  (Program NoTies NoTypedInstances) :: emptyReactEnv; emptyPlaceEnv; testGamma1; Peer "_" |- lambda (Id "x") Unit (idApp (Id "x")) : Unit ~> Unit.
 Proof. apply T_Abs. apply T_Var. left. reflexivity. Qed.
 
 
 Example test_hasType_TApp_1:
-  noPeers; noTies; emptyReactEnv; emptyPlaceEnv; emptyVarEnv; Peer "dummy" |- app (lambda (Id "x") Unit unit) unit : Unit.
+  (Program NoTies NoTypedInstances) :: emptyReactEnv; emptyPlaceEnv; emptyVarEnv; Peer "dummy" |- app (lambda (Id "x") Unit unit) unit : Unit.
 Proof.
   apply T_App with (T2 := Unit).
   - apply T_Abs. apply T_Unit.
@@ -92,7 +82,7 @@ Qed.
 
 
 Example test_hasType_TApp_2: 
-  noPeers; noTies; emptyReactEnv; emptyPlaceEnv; emptyVarEnv; Peer "dummy" |- app (lambda (Id "x") Unit (idApp (Id "x"))) unit : Unit.
+  (Program NoTies NoTypedInstances) :: emptyReactEnv; emptyPlaceEnv; emptyVarEnv; Peer "dummy" |- app (lambda (Id "x") Unit (idApp (Id "x"))) unit : Unit.
 Proof.
   apply T_App with (T2 := Unit).
   - apply T_Abs. apply T_Var. left. reflexivity.
@@ -101,12 +91,12 @@ Qed.
 
 
 Example test_hasType_TNil_1: 
-  noPeers; noTies; emptyReactEnv; emptyPlaceEnv; emptyVarEnv; Peer "dummy" |- nil Unit : List Unit.
+  (Program NoTies NoTypedInstances) :: emptyReactEnv; emptyPlaceEnv; emptyVarEnv; Peer "dummy" |- nil Unit : List Unit.
 Proof. apply T_Nil. Qed.
 
 
 Example test_hasType_TCons_1: 
-  noPeers; noTies; emptyReactEnv; emptyPlaceEnv; emptyVarEnv; Peer "dummy" |- cons unit (nil Unit) : List Unit.
+  (Program NoTies NoTypedInstances) :: emptyReactEnv; emptyPlaceEnv; emptyVarEnv; Peer "dummy" |- cons unit (nil Unit) : List Unit.
 Proof.
   apply T_Cons.
   - apply T_Unit.
@@ -115,17 +105,17 @@ Qed.
 
 
 Example test_hasType_TSome_1: 
-    noPeers; noTies; emptyReactEnv; emptyPlaceEnv; emptyVarEnv; Peer "dummy" |- some unit : Option Unit.
+    (Program NoTies NoTypedInstances) :: emptyReactEnv; emptyPlaceEnv; emptyVarEnv; Peer "dummy" |- some unit : Option Unit.
 Proof. apply T_Some. apply T_Unit. Qed.
 
 
 Example test_hasType_TNone_1: 
-    noPeers; noTies; emptyReactEnv; emptyPlaceEnv; emptyVarEnv; Peer "dummy" |- none Unit : Option Unit.
+    (Program NoTies NoTypedInstances) :: emptyReactEnv; emptyPlaceEnv; emptyVarEnv; Peer "dummy" |- none Unit : Option Unit.
 Proof. apply T_None. Qed.
 
 
 Example test_hasType_TPeer_1:
-  testPeerTyping1; testTies1; emptyReactEnv; emptyPlaceEnv; emptyVarEnv; Peer "p0" |- peerApp (PeerInst 0) : Remote (Peer "p0").
+  (Program testTies1 testPeerTyping1) :: emptyReactEnv; emptyPlaceEnv; emptyVarEnv; Peer "p0" |- peerApp (PeerInst 0) : Remote (Peer "p0").
 Proof. apply T_Peer. reflexivity. Qed.
 
 
@@ -133,7 +123,7 @@ Example test_hasType_TAsLocal_single_1:
   (* ensure test setup is correct ... *)
   testTies1 (Peer "p0", Peer "ps") = Some single /\
   (* actual test ... *)
-  noPeers; testTies1; emptyReactEnv; emptyPlaceEnv; emptyVarEnv; Peer "p0"
+  (Program testTies1 NoTypedInstances) :: emptyReactEnv; emptyPlaceEnv; emptyVarEnv; Peer "p0"
     |- asLocal unit (Unit on (Peer "ps")) : Unit.
 Proof.
   split.
@@ -150,7 +140,7 @@ Example test_hasType_TAsLocal_optional_1:
   (* ensure test setup is correct ... *)
   testTies1 (Peer "p0", Peer "po") = Some optional /\
   (* actual test ... *)
-  noPeers; testTies1; emptyReactEnv; emptyPlaceEnv; emptyVarEnv; Peer "p0"
+  (Program testTies1 NoTypedInstances) :: emptyReactEnv; emptyPlaceEnv; emptyVarEnv; Peer "p0"
     |- asLocal unit (Unit on (Peer "po")) : Option Unit.
 Proof.
   split.
@@ -167,7 +157,7 @@ Example test_hasType_TAsLocal_multiple_1:
   (* ensure test setup is correct ... *)
   testTies1 (Peer "p0", Peer "pm") = Some multiple /\
   (* actual test ... *)
-  noPeers; testTies1; emptyReactEnv; emptyPlaceEnv; emptyVarEnv; Peer "p0"
+  (Program testTies1 NoTypedInstances) :: emptyReactEnv; emptyPlaceEnv; emptyVarEnv; Peer "p0"
     |- asLocal unit (Unit on (Peer "pm")) : List Unit.
 Proof.
   split.
@@ -182,10 +172,10 @@ Qed.
 
 Example test_hasType_TAsLocalFrom_single_1:
   (* ensure test setup is correct ... *)
-  testPeerTyping1 (PeerInst 2) = Some (Peer "ps") /\
+  typed_peer_instances_type testPeerTyping1 (PeerInst 2) = Some (Peer "ps") /\
   testTies1 (Peer "p0", Peer "ps") = Some single /\
   (* actual test ... *)
-  testPeerTyping1; testTies1; emptyReactEnv; emptyPlaceEnv; emptyVarEnv; Peer "p0"
+  (Program testTies1 testPeerTyping1) :: emptyReactEnv; emptyPlaceEnv; emptyVarEnv; Peer "p0"
     |- asLocalFrom unit (Unit on (Peer "ps")) (peerApp (PeerInst 2)) : Unit.
 Proof.
   split.
@@ -202,10 +192,10 @@ Qed.
 
 Example test_hasType_TAsLocalFrom_optional_1:
   (* ensure test setup is correct ... *)
-  testPeerTyping1 (PeerInst 3) = Some (Peer "po") /\
+  typed_peer_instances_type testPeerTyping1 (PeerInst 3) = Some (Peer "po") /\
   testTies1 (Peer "p0", Peer "po") = Some optional /\
   (* actual test ... *)
-  testPeerTyping1; testTies1; emptyReactEnv; emptyPlaceEnv; emptyVarEnv; Peer "p0"
+  (Program testTies1 testPeerTyping1) :: emptyReactEnv; emptyPlaceEnv; emptyVarEnv; Peer "p0"
     |- asLocalFrom unit (Unit on (Peer "po")) (peerApp (PeerInst 3)) : Unit.
 Proof.
   split.
@@ -222,10 +212,10 @@ Qed.
 
 Example test_hasType_TAsLocalFrom_multiple_1:
   (* ensure test setup is correct ... *)
-  testPeerTyping1 (PeerInst 4) = Some (Peer "pm") /\
+  typed_peer_instances_type testPeerTyping1 (PeerInst 4) = Some (Peer "pm") /\
   testTies1 (Peer "p0", Peer "pm") = Some multiple /\
   (* actual test ... *)
-  testPeerTyping1; testTies1; emptyReactEnv; emptyPlaceEnv; emptyVarEnv; Peer "p0"
+  (Program testTies1 testPeerTyping1) :: emptyReactEnv; emptyPlaceEnv; emptyVarEnv; Peer "p0"
     |- asLocalFrom unit (Unit on (Peer "pm")) (peerApp (PeerInst 4)) : Unit.
 Proof.
   split.
@@ -244,7 +234,7 @@ Example test_hasType_TComp_single_1:
   (* ensure test setup is correct ... *)
   testTies1 (Peer "p0", Peer "ps") = Some single /\
   (* actual test ... *)
-  noPeers; testTies1; emptyReactEnv; emptyPlaceEnv; emptyVarEnv; Peer "p0"
+  (Program testTies1 NoTypedInstances) :: emptyReactEnv; emptyPlaceEnv; emptyVarEnv; Peer "p0"
     |- asLocalIn (Id "x") unit unit (Unit on (Peer "ps")) : Unit.
 Proof.
   split.
@@ -263,7 +253,7 @@ Example test_hasType_TComp_optional_1:
   (* ensure test setup is correct ... *)
   testTies1 (Peer "p0", Peer "po") = Some optional /\
   (* actual test ... *)
-  noPeers; testTies1; emptyReactEnv; emptyPlaceEnv; emptyVarEnv; Peer "p0"
+  (Program testTies1 NoTypedInstances) :: emptyReactEnv; emptyPlaceEnv; emptyVarEnv; Peer "p0"
     |- asLocalIn (Id "x") unit unit (Unit on (Peer "po")) : Option Unit.
 Proof.
   split.
@@ -282,7 +272,7 @@ Example test_hasType_TComp_multiple_1:
   (* ensure test setup is correct ... *)
   testTies1 (Peer "p0", Peer "pm") = Some multiple /\
   (* actual test ... *)
-  noPeers; testTies1; emptyReactEnv; emptyPlaceEnv; emptyVarEnv; Peer "p0"
+  (Program testTies1 NoTypedInstances) :: emptyReactEnv; emptyPlaceEnv; emptyVarEnv; Peer "p0"
     |- asLocalIn (Id "x") unit unit (Unit on (Peer "pm")) : List Unit.
 Proof.
   split.
@@ -301,7 +291,7 @@ Example test_hasType_TComp_single_2:
   (* ensure test setup is correct ... *)
   testTies1 (Peer "p0", Peer "ps") = Some single /\
   (* actual test ... *)
-  noPeers; testTies1; emptyReactEnv; emptyPlaceEnv; emptyVarEnv; Peer "p0"
+  (Program testTies1 NoTypedInstances) :: emptyReactEnv; emptyPlaceEnv; emptyVarEnv; Peer "p0"
     |- asLocalIn (Id "x") unit (idApp (Id "x")) (Unit on (Peer "ps")) : Unit.
 Proof.
   split.
@@ -318,10 +308,10 @@ Qed.
 
 Example test_hasType_TCompFrom_single_1:
   (* ensure test setup is correct ... *)
-  testPeerTyping1 (PeerInst 2) = Some (Peer "ps") /\
+  typed_peer_instances_type testPeerTyping1 (PeerInst 2) = Some (Peer "ps") /\
   testTies1 (Peer "p0", Peer "ps") = Some single /\
   (* actual test ... *)
-  testPeerTyping1; testTies1; emptyReactEnv; emptyPlaceEnv; emptyVarEnv; Peer "p0"
+  (Program testTies1 testPeerTyping1) :: emptyReactEnv; emptyPlaceEnv; emptyVarEnv; Peer "p0"
     |- asLocalInFrom (Id "x") (*=*) unit (*in*) unit (*:*) (Unit on (Peer "ps"))
                      (*from*) (peerApp (PeerInst 2))
     : Unit.
@@ -342,10 +332,10 @@ Qed.
 
 Example test_hasType_TCompFrom_single_2:
   (* ensure test setup is correct ... *)
-  testPeerTyping1 (PeerInst 2) = Some (Peer "ps") /\
+  typed_peer_instances_type testPeerTyping1 (PeerInst 2) = Some (Peer "ps") /\
   testTies1 (Peer "p0", Peer "ps") = Some single /\
   (* actual test ... *)
-  testPeerTyping1; testTies1; emptyReactEnv; emptyPlaceEnv; emptyVarEnv; Peer "p0"
+  (Program testTies1 testPeerTyping1) :: emptyReactEnv; emptyPlaceEnv; emptyVarEnv; Peer "p0"
     |- asLocalInFrom (Id "x") (*=*) unit (*in*) (idApp (Id "x"))
                      (*:*) (Unit on (Peer "ps"))
                      (*from*) (peerApp (PeerInst 2))
@@ -369,7 +359,7 @@ Example test_hasType_TReactive_1:
   (* ensure test setup is correct ... *)
   testPsi1 (Reactive 0) = Some Unit /\
   (* actual test ... *)
-  noPeers; noTies; testPsi1; emptyPlaceEnv; emptyVarEnv; Peer "_" |- reactApp (Reactive 0) : Unit.
+  (Program NoTies NoTypedInstances) :: testPsi1; emptyPlaceEnv; emptyVarEnv; Peer "_" |- reactApp (Reactive 0) : Unit.
 Proof.
   split.
   - reflexivity.
@@ -378,17 +368,17 @@ Qed.
 
 
 Example test_hasType_TSignal_1:
-  noPeers; noTies; emptyReactEnv; emptyPlaceEnv; emptyVarEnv; Peer "dummy" |- signal unit : Signal Unit.
+  (Program NoTies NoTypedInstances) :: emptyReactEnv; emptyPlaceEnv; emptyVarEnv; Peer "dummy" |- signal unit : Signal Unit.
 Proof. apply T_Signal. apply T_Unit. Qed.
 
 
 Example test_hasType_TReactiveVal_1:
-  noPeers; noTies; emptyReactEnv; emptyPlaceEnv; emptyVarEnv; Peer "dummy" |- var unit : Var Unit.
+  (Program NoTies NoTypedInstances) :: emptyReactEnv; emptyPlaceEnv; emptyVarEnv; Peer "dummy" |- var unit : Var Unit.
 Proof. apply T_ReactiveVar. apply T_Unit. Qed.
 
 
 Example test_hasType_TNow_signal_1:
-  noPeers; noTies; emptyReactEnv; emptyPlaceEnv; emptyVarEnv; Peer "dummy" |- now (signal unit) : Unit.
+  (Program NoTies NoTypedInstances) :: emptyReactEnv; emptyPlaceEnv; emptyVarEnv; Peer "dummy" |- now (signal unit) : Unit.
 Proof.
   apply T_Now with (T0 := Signal Unit).
   - apply T_Signal. apply T_Unit.
@@ -397,7 +387,7 @@ Qed.
 
 
 Example test_hasType_TNow_var_1:
-  noPeers; noTies; emptyReactEnv; emptyPlaceEnv; emptyVarEnv; Peer "dummy" |- now (var unit) : Unit.
+  (Program NoTies NoTypedInstances) :: emptyReactEnv; emptyPlaceEnv; emptyVarEnv; Peer "dummy" |- now (var unit) : Unit.
 Proof.
   eapply T_Now.
   - apply T_ReactiveVar. apply T_Unit.
@@ -406,7 +396,7 @@ Qed.
 
 
 Example test_hasType_TSet_1:
-  noPeers; noTies; emptyReactEnv; emptyPlaceEnv; emptyVarEnv; Peer "dummy" |- set (var unit) unit : Unit.
+  (Program NoTies NoTypedInstances) :: emptyReactEnv; emptyPlaceEnv; emptyVarEnv; Peer "dummy" |- set (var unit) unit : Unit.
 Proof.
   apply T_Set with (T := Unit).
   - apply T_ReactiveVar. apply T_Unit.
@@ -415,12 +405,12 @@ Qed.
 
 
 Example test_hasType_TSet_2:
-  noPeers; noTies; emptyReactEnv; emptyPlaceEnv; emptyVarEnv; Peer "dummy"
+  (Program NoTies NoTypedInstances) :: emptyReactEnv; emptyPlaceEnv; emptyVarEnv; Peer "dummy"
     |- set (var (lambda (Id "x") Unit unit))
            (*:=*) (lambda (Id "x") Unit unit)
     : Unit.
 Proof.
-  assert (H: noPeers; noTies; emptyReactEnv; emptyPlaceEnv; emptyVarEnv; Peer "dummy" |- lambda (Id "x") Unit unit : Unit ~> Unit).
+  assert (H: (Program NoTies NoTypedInstances) :: emptyReactEnv; emptyPlaceEnv; emptyVarEnv; Peer "dummy" |- lambda (Id "x") Unit unit : Unit ~> Unit).
   - apply T_Abs.
     apply T_Unit.
   - apply T_Set with (T := Unit ~> Unit).
